PREFIX lcn: <https://data.idnau.org/pid/vocab/lc-notices/>
PREFIX lcncs: <https://data.idnau.org/pid/vocab/lc-notices>
PREFIX dcterms: <http://purl.org/dc/terms/>
PREFIX lcont: <https://data.idnau.org/pid/lc-ont/>
PREFIX odrl: <http://www.w3.org/ns/odrl/2/>
PREFIX owl: <http://www.w3.org/2002/07/owl#>
PREFIX rdfs: <http://www.w3.org/2000/01/rdf-schema#>
PREFIX sdo: <https://schema.org/>
PREFIX skos: <http://www.w3.org/2004/02/skos/core#>
PREFIX xsd: <http://www.w3.org/2001/XMLSchema#>


lcncs:
    a skos:ConceptScheme ;
    skos:prefLabel "Local Contexts Notices"@en ;
    skos:definition "The Notices are tools for institutions and researchers to identify Indigenous collections and data and recognize Indigenous rights and interests. The Notices were developed to create pathways for partnership, collaboration, and support of Indigenous cultural authority."@en ;
    sdo:citation "https://localcontexts.org/notices/about-the-notices/"@en ;
    dcterms:creator <https://kurrawong.ai> ;
    dcterms:created "2026-02-11"^^xsd:date ;
    sdo:dateCreated "2026-02-11"^^xsd:date ;
    sdo:dateModified "2026-02-11"^^xsd:date ;
    owl:versionInfo "0.1" ;
    skos:hasTopConcept lcn:open-to-collaboration , lcn:attribution-incomplete , lcn:tk-notice , lcn:bc-notice , lcn:authorization , lcn:belonging , lcn:caring , lcn:gender-aware , lcn:leave-undisturbed , lcn:safety , lcn:viewing , lcn:withholding
.

# lc notice concept collections

lcn:collection-engage
    a skos:Collection ;
    skos:prefLabel "Local Contexts Engagement Notice collection"@en ;
    skos:definition "A collection of Local Contexts engagement notices"@en ;
    sdo:citation "https://localcontexts.org/notice/open-to-collaborate/"^^xsd:anyURI ;
    dcterms:creator <https://kurrawong.ai> ;
    dcterms:created "2026-02-11"^^xsd:date ;
    sdo:dateCreated "2026-02-11"^^xsd:date ;
    sdo:dateModified "2026-02-12"^^xsd:date ;
    owl:versionInfo "0.1" ;
    skos:member lcn:open-to-collaboration
.

lcn:collection-disclosure
    a skos:Collection ;
    skos:prefLabel "Local Contexts Discosulre Notice collection"@en ;
    skos:definition "A collection of Local Contexts disclosure notices"@en ;
    sdo:citation "https://localcontexts.org/notices/disclosure-notices/"^^xsd:anyURI ;
    dcterms:creator <https://kurrawong.ai> ;
    dcterms:created "2026-02-11"^^xsd:date ;
    sdo:dateCreated "2026-02-11"^^xsd:date ;
    sdo:dateModified "2026-02-11"^^xsd:date ;
    owl:versionInfo "0.1" ;
    skos:member
       lcn:attribution-incomplete ,
       lcn:tk-notice ,
       lcn:bc-notice
.

lcn:collection-collections-care
    a skos:Collection ;
    skos:prefLabel "Local Contexts Collections Care Notice collection"@en ;
    skos:definition "A collection of Local Contexts collections care notices"@en ;
    sdo:citation "https://localcontexts.org/notices/cc-notices/"^^xsd:anyURI ;
    dcterms:creator <https://kurrawong.ai> ;
    dcterms:created "2026-02-11"^^xsd:date ;
    sdo:dateCreated "2026-02-11"^^xsd:date ;
    sdo:dateModified "2026-02-11"^^xsd:date ;
    owl:versionInfo "0.1" ;
    skos:member
       lcn:authorization ,
       lcn:belonging ,
       lcn:caring ,
       lcn:gender-aware ,
       lcn:leave-undisturbed ,
       lcn:safety ,
       lcn:viewing ,
       lcn:withholding
.

# concepts

lcn:attribution-incomplete 
    a lcont:LCNotice, skos:Concept , odrl:Policy ;
    skos:prefLabel ""@en ;
    skos:definition "The Attribution Incomplete Notice is attached to a collection or at an item level where there is incomplete, inaccurate, or missing attribution. This Notice indicates to the public that the record and/or metadata is incomplete. Visibly identifying missing attribution within collections is the first step towards correcting existing attribution to include: contributors, collaborators, other authors and/or communities of origin."@en ;
    dcterms:identifier "authorization-incomplete"^^xsd:token ;
    lcont:templateText "Collections and items in our institution have incomplete, inaccurate, and/or missing attribution. We are using this notice to clearly identify this material so that it can be updated, or corrected by communities of origin. Our institution is committed to collaboration and partnerships to address this problem of incorrect or missing attribution."@en ;
    sdo:citation "https://localcontexts.org/notice/attribution-incomplete/"^^xsd:anyURI ;
    skos:inScheme lcncs: ;
    skos:topConceptOf lcncs: ;
.

lcn:authorization
    a lcont:LCNotice, skos:Concept , odrl:Policy ;
    skos:prefLabel "Authorization"@en ;
    skos:definition "The Authorization Notice recognizes that specific Tribal or community authorization through consultation is necessary prior to use of specific items or collections in all forms of publication and exhibits."@en ;
    dcterms:identifier "authorization"^^xsd:token ;
    lcont:templateText "The Authorization Notice is being used to indicate that distinct Tribal or community authorization through consultation needs to be obtained for any reproduction of this item, including for the use in exhibitions and publications in print or online."@en ;
    sdo:citation "https://localcontexts.org/notice/authorization/"^^xsd:anyURI ;
    skos:inScheme lcncs: ;
    skos:topConceptOf lcncs: ;
.

#######
# to do

lcn:bc-notice
   a lcont:LCNotice, skos:Concept , odrl:Policy ;
    skos:prefLabel "BC Notice"@en ;
    skos:definition ""@en ;
    dcterms:identifier "bc-notice"^^xsd:token ;
    lcont:templateText ""@en ;
    sdo:citation "https://localcontexts.org/notice/authorization/"^^xsd:anyURI ;
    skos:inScheme lcncs: ;
    skos:topConceptOf lcncs: ;
.
#######

lcn:belonging
   a lcont:LCNotice, skos:Concept , odrl:Policy ;
    skos:prefLabel "Belonging"@en ;
    skos:definition "The Belonging Notice recognizes the exclusive right of Indigenous communities, Tribes, Clans, or societies to access and handle items or collections."@en ;
    dcterms:identifier "belonging"^^xsd:token ;
    lcont:templateText "The Belonging Notice is being used to indicate that only specific persons belonging to communities, Tribes, Clans, and societies have the right to access and handle these specific items or collections."@en ;
    sdo:citation "https://localcontexts.org/notice/belonging/"^^xsd:anyURI ;
    skos:inScheme lcncs: ;
    skos:topConceptOf lcncs: ;
.

lcn:caring
   a lcont:LCNotice, skos:Concept , odrl:Policy ;
    skos:prefLabel "Caring"@en ;
    skos:definition "The Caring Notice recognizes cultural ways of caring for materials including specific ways of handling, storing, or managing specific items or collections. In all cases, care will be defined through community consultations."@en ;
    dcterms:identifier "caring"^^xsd:token ;
    lcont:templateText "The Caring Notice is being used to indicate that specialized cultural care is required. Care for items or collections will require specific community guidelines for storage and handling."@en ;
    sdo:citation "https://localcontexts.org/notice/caring/"^^xsd:anyURI ;
    skos:inScheme lcncs: ;
    skos:topConceptOf lcncs: ;
.


lcn:gender-aware 

lcn:leave-undisturbed


lcn:open-to-collaboration ,  lcn:tk-notice , lcn:safety , lcn:viewing , lcn:withholding




# to do: add below to lc-ont

lcont:LCNotice
    a owl:Class ;
    rdfs:isDefinedBy ont: ;
    sdo:description The class of all Notice concepts from the Local Contexts framework." ;
    sdo:name "Local Contexts Notice" ;
.

