prefix : <https://data.idnau.org/pid/system/>
prefix aarr: <https://data.idnau.org/pid/vocab/aarr/>
prefix cs: <https://data.idnau.org/pid/system>
prefix adb: <https://data.idnau.org/pid/adb/>
prefix skos: <http://www.w3.org/2004/02/skos/core#>
prefix xsd: <http://www.w3.org/2001/XMLSchema#>
prefix dcterms: <http://purl.org/dc/terms/>
prefix id: <http://id.loc.gov/vocabulary/identifiers/>
prefix sdo: <https://schema.org/>
prefix dcat: <http://www.w3.org/ns/dcat#>
prefix prov: <http://www.w3.org/ns/prov#>
prefix aarr: <https://data.idnau.org/pid/vocab/aarr/>
prefix idncp: <https://data.idnau.org/pid/cp/>

<https://linked.data.gov.au/org/idn>
    a sdo:Organization ;
    dcterms:type <https://data.idnau.org/pid/vocab/org-indigeneity/non-indigenous> ;
    dcat:qualifiedRelation [
            dcat:hadRole aarr:partOf ;
            sdo:agent <https://data.idnau.org/pid/org/isu>
        ] ;
    sdo:description "The IDN is within the University of Melbourne. It was established in 2018 to support and coordinate the governance of Indigenous data for Aboriginal and Torres Strait Islander peoples and empower Aboriginal and Torres Strait Islander communities to decide their own local data priorities." ;
    sdo:name "Indigenous Data Network" ;
    sdo:url "https://mspgh.unimelb.edu.au/centres-institutes/centre-for-health-equity/research-group/indigenous-data-network"^^xsd:anyURI ;
.

<https://kurrawong.ai>
    a sdo:Organization ;
    dcterms:type <https://data.idnau.org/pid/vocab/org-indigeneity/non-indigenous> ;
    sdo:description "Kurrawong AI is a small, Artificial Intelligence, company in Australia specialising in Knowledge Graphs." ;
    sdo:identifier "31353542036"^^id:ausbn ;
    sdo:name "KurrawongAI" ;
    sdo:url "https://kurrawong.ai"^^xsd:anyURI ;
.

:oric a skos:Concept ;
	skos:prefLabel "ORIC" ;
	skos:definition "Office of the Registrar of Indigenous Corporations" ;
	skos:scopeNote """
	By definition the ORIC system contains only Indigenous corporations.
	Registered corporations can be found by searching the main site.
	An extract of the ORIC system is included in the IDN agents database.""" ;
	dcterms:source "https://www.oric.gov.au/corporations-and-registers/find-corporation"^^xsd:anyURI ;
	skos:inScheme cs: ;
.

:orcid a skos:Concept ;
	skos:prefLabel "ORCID" ;
	skos:definition "Open Researcher and Contributor ID" ;
	skos:scopeNote """
	The ORCID system is a global not-for-profit that provides identifiers for researchers and contributors.
	ORCID is not exclusively for listing Indigenous agents but can be filtered by using the Indigenous Studies keyword.
	""" ;
	dcterms:source "https://orcid.org/orcid-search/search?keyword=Indigenous%20Studies"^^xsd:anyURI ;
	skos:inScheme cs: ;
.

:find-an-expert a skos:Concept ;
	skos:prefLabel "Find an Expert" ;
	skos:definition "University of Melbourne's Find an Expert system." ;
	skos:scopeNote """
	The Find an Expert system is a service provided by the University of Melbourne. While it is not exclusively a register
	of Indigenous agents, it is a useful resource for communities to find Indigenous experts.
	The Find an Expert system can be filtered to show Indigenous agents using the Indigenous Studies category.
	""" ;
	dcterms:source "https://findanexpert.unimelb.edu.au/searchresults?q=Indigenous%20studies&category=profile"^^xsd:anyURI ;
	skos:inScheme cs: ;
.

cs: a skos:ConceptScheme ;
	skos:prefLabel "External Agentic systems" ;
	skos:definition "List of external systems holding Indigenous agents." ;
	skos:scopeNote "The aim of this vocabulary is to aid and inform the discovery of Indigenous agents from external systems." ;
	skos:historyNote "Created by hand for the IDN agents database." ;
	dcterms:publisher <https://linked.data.gov.au/org/idn> ;
	dcterms:creator <https://kurrawong.ai> ;
	dcterms:created "2024-11-01"^^xsd:date ;
	dcterms:modified "2024-11-01"^^xsd:date ;
	skos:hasTopConcept
		:oric
.

