PREFIX cs: <https://linked.data.gov.au/def/data-access-rights>
PREFIX : <https://linked.data.gov.au/def/data-access-rights/>
PREFIX dcterms: <http://purl.org/dc/terms/>
PREFIX owl: <http://www.w3.org/2002/07/owl#>
PREFIX prov: <http://www.w3.org/ns/prov#>
PREFIX rdfs: <http://www.w3.org/2000/01/rdf-schema#>
PREFIX reg: <http://purl.org/linked-data/registry#>
PREFIX sdo: <https://schema.org/>
PREFIX skos: <http://www.w3.org/2004/02/skos/core#>
PREFIX xsd: <http://www.w3.org/2001/XMLSchema#>

:closed-access-rights
    a skos:Collection ;
    rdfs:isDefinedBy cs: ;
    skos:definition "Selective restriction of access to data that is OFFICIAL (low or negligible confidentiality impact), SENSITIVE (moderate confidentiality impact) or PROTECTED (high confidentiality impact)."@en ;
    skos:historyNote "Added by the Geological Survey of Queensland, 2018" ;
    skos:inScheme cs: ;
    skos:member
        :conditional ,
        :embargoed ,
        :metadata-only ,
        :protected ,
        :restricted ;
    skos:prefLabel "Closed data access rights"@en ;
.

:open-access-rights
    a skos:Collection ;
    rdfs:isDefinedBy cs: ;
    skos:definition "Data that is non-sensitive, freely available, easily discovered and accessed, and published in ways and with licences that allow easy reuse."@en ;
    skos:historyNote "Added by the Geological Survey of Queensland, 2018" ;
    skos:inScheme cs: ;
    skos:member :open ;
    skos:prefLabel "Open data access rights"@en ;
.

:conditional
    a skos:Concept ;
    skos:definition "Conditionally protected access refers to a resource that is stored in a system but is not freely accessible and remains protected based on the satisfaction of other specified criteria. Access is limited to specific personnel or user groups. "@en ;
    skos:historyNote "Original term in the COAR vocabulary" ;
    skos:inScheme cs: ;
    skos:prefLabel "Conditionally protected"@en ;
    skos:narrower :metadata-only ;
.

:embargoed
    a skos:Concept ;
    skos:definition "Embargoed access refers to a resource accessible as metadata only until released for open access on a specified date."@en ;
    skos:historyNote "Original term in the COAR vocabulary" ;
    skos:inScheme cs: ;
    skos:prefLabel "Embargoed access"@en ;
.

:metadata-only
    a skos:Concept ;
    skos:definition "Metadata only access refers to a resource in which access is limited to metadata only. Access to the resource requires granting of access rights."@en ;
    skos:historyNote "Original term in the COAR vocabulary" ;
    skos:inScheme cs: ;
    skos:prefLabel "Metadata only access"@en ;
.

:open
    a skos:Concept ;
    skos:altLabel "Open file"@en ;
    skos:definition "Open access refers to a resource that is immediately and permanently online, and free for all on the Web, without financial and technical barriers."@en ;
    skos:historyNote "Original term in the COAR vocabulary" ;
    skos:inScheme cs: ;
    skos:prefLabel "Open access"@en ;
    skos:topConceptOf cs: ;
.

:protected
    a skos:Concept ;
    skos:definition "Protected access refers to a resource that is stored in a system but is not freely accessible due to specific legal or policy decisions, such as active legal proceedings or ministerial discretion. Access is limited to specific personnel or user groups. "@en ;
    skos:historyNote "Original term in the COAR vocabulary" ;
    skos:inScheme cs: ;
    skos:prefLabel "Protected access"@en ;
.

:restricted
    a skos:Concept ;
    skos:definition "Restricted access refers to a resource that is stored in a system but is not freely accessible. Access is limited to specific personnel or user groups."@en ;
    skos:historyNote "Original term in the COAR vocabulary" ;
    skos:inScheme cs: ;
    skos:prefLabel "Restricted access"@en ;
    skos:topConceptOf cs: ;
    skos:narrower
        :protected ,
        :conditional ,
        :embargoed ,
        :limited-community-access ;
.

:limited-communities-access
    a skos:Concept ;
    reg:status <https://linked.data.gov.au/def/reg-statuses/addition> ;
    skos:definition "Access is limited to particular communities only"@en ;
    skos:historyNote "Created by the Indigenous Data Network, 2024" ;
    skos:inScheme cs: ;
    skos:prefLabel "Limited Communities Access"@en ;
    skos:narrower :indigenous-communities-access ;
.

:indigenous-communities-access
    a skos:Concept ;
    reg:status <https://linked.data.gov.au/def/reg-statuses/addition> ;
    skos:definition "Access is limited to particular indigenous communities only"@en ;
    skos:historyNote "Created by the Indigenous Data Network, 2024" ;
    skos:inScheme cs: ;
    skos:prefLabel "Indigenous Communities Access"@en ;
.

<https://linked.data.gov.au/org/gsq>
    a sdo:Organization ;
    sdo:name "Geological Survey of Queensland" ;
    sdo:url "http://www.business.qld.gov.au/industries/mining-energy-water/resources/geoscience-information/gsq"^^xsd:anyURI ;
.

cs:
    a
        owl:Ontology ,
        skos:ConceptScheme ;
    dcterms:created "2019-04-03"^^xsd:date ;
    dcterms:creator <https://linked.data.gov.au/org/gsq> ;
    dcterms:modified "2021-02-08"^^xsd:date ;
    dcterms:publisher <https://linked.data.gov.au/org/gsq> ;
    dcterms:source "http://vocabularies.coar-repositories.org/documentation/access_rights/"^^xsd:anyURI ;
    reg:status <https://linked.data.gov.au/def/reg-statuses/stable> ;
    skos:definition "Data access rights control how users and systems access a data resource."@en ;
    skos:historyNote "This vocabulary is taken from the COAR Controlled Vocabularies Interest Group (http://vocabularies.coar-repositories.org/documentation/access_rights/) but is redelivered as that vocabulary isn't well presented online."@en ;
    skos:prefLabel "Data Access Rights"@en ;
    skos:hasTopConcept
        :open ,
        :restricted ;
    prov:qualifiedDerivation [
        prov:entity cs: ;
        prov:hadRole <https://linked.data.gov.au/def/vocdermods/none> ;
    ] ;
.
