PREFIX : <https://data.idnau.org/pid/glossary/>
PREFIX cs: <https://data.idnau.org/pid/glossary>
PREFIX dcat: <http://www.w3.org/ns/dcat#>
PREFIX isoroles: <https://linked.data.gov.au/def/data-roles/>
PREFIX owl: <http://www.w3.org/2002/07/owl#>
PREFIX prov: <http://www.w3.org/ns/prov#>
PREFIX rdfs: <http://www.w3.org/2000/01/rdf-schema#>
PREFIX schema: <https://schema.org/>
PREFIX skos: <http://www.w3.org/2004/02/skos/core#>
PREFIX xsd: <http://www.w3.org/2001/XMLSchema#>

:021c5daa-1354-4dd5-b8cf-8eb112e09174
    a skos:Concept ;
    rdfs:isDefinedBy cs: ;
    skos:definition "Tracking changes to resources over time."@en ;
    skos:inScheme cs: ;
    skos:prefLabel "Versioning"@en ;
    skos:topConceptOf cs: ;
.

:2cab7bd9-8e6d-408b-8120-58ebf0953607
    a skos:Concept ;
    rdfs:isDefinedBy cs: ;
    skos:definition "A resource is accessible if it is possible to get a resource by a persistant identifier, or to get information about how to get the resource."@en ;
    skos:inScheme cs: ;
    skos:prefLabel "Accessible"@en ;
    skos:topConceptOf cs: ;
.

:324b9d70-1d31-450a-bc5e-a91ab7d65875
    a skos:Concept ;
    rdfs:isDefinedBy cs: ;
    skos:altLabel "RDF@en"@en ;
    skos:definition "A type of metadata for describing resources on the internet."@en ;
    skos:inScheme cs: ;
    skos:prefLabel "Resource Description Framework"@en ;
    skos:topConceptOf cs: ;
    schema:citation "https://www.w3.org/TR/rdf11-concepts/"^^xsd:anyURI ;
.

:37258c00-fea6-4837-8b3c-db9efa85a4e3
    a skos:Concept ;
    rdfs:isDefinedBy cs: ;
    skos:definition "A tool that checks if metadata conforms to the rules of a profile."@en ;
    skos:inScheme cs: ;
    skos:prefLabel "Validator"@en ;
    skos:topConceptOf cs: ;
    schema:citation "https://data.idnau.org/pid/cp/validator/"^^xsd:anyURI ;
.

:37e0be20-e754-4f7c-a7c8-cb769e3b8d9d
    a skos:Concept ;
    rdfs:isDefinedBy cs: ;
    skos:definition "A set of rules or guidelines for creating consistent metadata."@en ;
    skos:inScheme cs: ;
    skos:prefLabel "Profile"@en ;
    skos:topConceptOf cs: ;
.

:3e4ebd2a-a787-44c7-b8b9-697e91df313d
    a skos:Concept ;
    rdfs:isDefinedBy cs: ;
    skos:altLabel
        "Catalog@en"@en ,
        "Data catalogue@en"@en ;
    skos:definition "A collection of metadata records organised for easy access and use."@en ;
    skos:inScheme cs: ;
    skos:prefLabel "Catalogue"@en ;
    skos:topConceptOf cs: ;
.

:5876f61f-1c82-4ac8-894b-b2bfc4debf8d
    a skos:Concept ;
    rdfs:isDefinedBy cs: ;
    skos:altLabel "Interoperable@en"@en ;
    skos:definition "The ability to share information between different collections or catalogues that might use different tools."@en ;
    skos:inScheme cs: ;
    skos:prefLabel "Interoperability"@en ;
    skos:topConceptOf cs: ;
.

:61ee574a-e34e-4636-8d6f-5d7ce5807528
    a skos:Concept ;
    rdfs:isDefinedBy cs: ;
    skos:altLabel "JavaScript Object Notation for Linked Data@en"@en ;
    skos:definition "A method for storing and sharing Resource Description Framework metadata."@en ;
    skos:inScheme cs: ;
    skos:prefLabel "JSON-LD"@en ;
    skos:topConceptOf cs: ;
    schema:citation "https://json-ld.org"^^xsd:anyURI ;
.

:63da5279-8772-4f9c-8e55-6f5f6f85129a
    a skos:Concept ;
    rdfs:isDefinedBy cs: ;
    skos:definition "Metadata about the relationships between things."@en ;
    skos:inScheme cs: ;
    skos:prefLabel "Ontology"@en ;
    skos:topConceptOf cs: ;
.

:6ac34814-bd33-44ce-a1e9-5c71e88f8d06
    a skos:Concept ;
    rdfs:isDefinedBy cs: ;
    skos:definition "Principles to make resourcesÂ Findable, Accessible, Interoperable, and Reusable."@en ;
    skos:inScheme cs: ;
    skos:prefLabel "FAIR principles"@en ;
    skos:topConceptOf cs: ;
.

:6d0f3fed-3187-4825-ad06-35956922dada
    a skos:Concept ;
    rdfs:isDefinedBy cs: ;
    skos:altLabel
        "Concept scheme@en"@en ,
        "Controlled vocabulary@en"@en ;
    skos:definition "A set of predefined words or phrases used for describing metadata records consistently."@en ;
    skos:inScheme cs: ;
    skos:prefLabel "Vocabulary"@en ;
    skos:topConceptOf cs: ;
.

:6f057945-b9b9-41ac-b7c1-8eb739bee9fa
    a skos:Concept ;
    rdfs:isDefinedBy cs: ;
    skos:altLabel "DCAT@en"@en ;
    skos:definition "A standard used for describing data catalogs on the web to enable interoperability between systems."@en ;
    skos:inScheme cs: ;
    skos:prefLabel "Data Catalog Vocabulary"@en ;
    skos:topConceptOf cs: ;
    schema:citation "https://www.w3.org/TR/vocab-dcat-3/"^^xsd:anyURI ;
.

:81b2c6f3-1e8c-4a81-ab3b-7949dfc53456
    a skos:Concept ;
    rdfs:isDefinedBy cs: ;
    skos:definition "A resource is reuseable if there is permission from those responsible for the resource to use it."@en ;
    skos:inScheme cs: ;
    skos:prefLabel "Reuseable"@en ;
    skos:topConceptOf cs: ;
.

:87931538-66e5-493d-800f-3c8a54fb8d6b
    a skos:Concept ;
    rdfs:isDefinedBy cs: ;
    skos:definition "The prefix of an identifeir that groups concepts or resources together."@en ;
    skos:inScheme cs: ;
    skos:prefLabel "Namespace"@en ;
    skos:topConceptOf cs: ;
.

:8949db57-af31-47fb-a089-b0a77e3feb0e
    a skos:Concept ;
    rdfs:isDefinedBy cs: ;
    skos:definition "Information that describes a resource, such as its title, description, author or custodian."@en ;
    skos:inScheme cs: ;
    skos:prefLabel "Metadata"@en ;
    skos:topConceptOf cs: ;
.

:9c8ca3b5-cf7d-4c73-83c1-c5c7e5cabb9f
    a skos:Concept ;
    rdfs:isDefinedBy cs: ;
    skos:altLabel "Terse RDF Triple Language@en"@en ;
    skos:definition "A method for storing and sharing Resource Description Framework metadata."@en ;
    skos:inScheme cs: ;
    skos:prefLabel "Turtle"@en ;
    skos:topConceptOf cs: ;
    schema:citation "https://www.w3.org/TR/turtle/"^^xsd:anyURI ;
.

:a06424dd-4d26-4f01-85ee-ca8ff5dfc641
    a skos:Concept ;
    rdfs:isDefinedBy cs: ;
    skos:definition "The relationship between people or organisations and catalogued resources."@en ;
    skos:inScheme cs: ;
    skos:prefLabel "Role"@en ;
    skos:topConceptOf cs: ;
.

:a5cac5df-9d31-4f06-bf2a-fc32bb403e6c
    a skos:Concept ;
    rdfs:isDefinedBy cs: ;
    skos:altLabel "UUID@en"@en ;
    skos:broader :6c014466-c95f-4df5-a6cc-a1a50beffab0 ;
    skos:definition "A type of persistant identifier that is universally unique."@en ;
    skos:inScheme cs: ;
    skos:prefLabel "Universally Unique Identifier"@en ;
.

:a877b16b-2581-4339-9da4-87774b14980a
    a skos:Concept ;
    rdfs:isDefinedBy cs: ;
    skos:altLabel
        "BC labels@en"@en ,
        "Bicultural labels@en"@en ,
        "LC labels@en"@en ,
        "Traditional knowledge labels@en"@en ;
    skos:definition "Conepts that express local and specific conditions such as community rules, governance and protocols for using and sharing knowledge."@en ;
    skos:inScheme cs: ;
    skos:prefLabel "Local context labels"@en ;
    skos:topConceptOf cs: ;
    schema:citation "https://localcontexts.org/labels/traditional-knowledge-labels/"^^xsd:anyURI ;
.

:ac5eba92-55dc-494c-9d9f-b331e05e7c8d
    a skos:Concept ;
    rdfs:isDefinedBy cs: ;
    skos:definition "A single unit of meaning or part of knowledge. Conepts are expressed as words or terms. Many concepts from the same knowledge system belong to a vocabulary."@en ;
    skos:inScheme cs: ;
    skos:prefLabel "Concept"@en ;
    skos:topConceptOf cs: ;
    schema:citation "https://www.w3.org/TR/skos-reference/#concepts"^^xsd:anyURI ;
.

:c22de8ec-914d-46c9-8c70-3c859765f43e
    a skos:Concept ;
    rdfs:isDefinedBy
        cs: ,
        isoroles:subjectAgent ;
    skos:broader :57110a82-2f4a-4038-aa71-4bbbc888aac4 ;
    skos:definition "Person or organisation that the resource is about."@en ;
    skos:inScheme cs: ;
    skos:prefLabel "Subject agent"@en ;
.

:c44493ef-8c87-4e41-ac6d-2a0961203a07
    a skos:Concept ;
    rdfs:isDefinedBy cs: ;
    skos:altLabel "Metadata tool@"@en ;
    skos:definition "A tool that helps to create and upload metadata about resources."@en ;
    skos:inScheme cs: ;
    skos:prefLabel "Metadata Entry Form" ;
    skos:topConceptOf cs: ;
.

:d7907201-7eaa-4c08-80e1-404c3c2af5c1
    a skos:Concept ;
    rdfs:isDefinedBy cs: ;
    skos:definition "A resource is findable if it is possible to find that resource. Resources are findable when they are described with consistent metadata and vocabulary concepts."@en ;
    skos:inScheme cs: ;
    skos:prefLabel "Findable"@en ;
    skos:topConceptOf cs: ;
.

:df76959d-d915-4ce6-9bc8-8043dabc0cc2
    a skos:Concept ;
    rdfs:isDefinedBy cs: ;
    skos:altLabel "Qualified attribution@en"@en ;
    skos:definition "Metadata about the agent and the role that they played with respect to a resource."@en ;
    skos:inScheme cs: ;
    skos:prefLabel "Attribution"@en ;
    skos:topConceptOf cs: ;
.

:e1d0f465-d5a9-4154-a241-60c187e825e2
    a skos:Concept ;
    rdfs:isDefinedBy cs: ;
    skos:definition "Priniples for the ethical use and sharing of data to prioritize community benefit, agency, and respect. They are: Collective Benefit; Authority to Control; Responsibility; Ethics."@en ;
    skos:inScheme cs: ;
    skos:prefLabel "CARE Principles"@en ;
    skos:topConceptOf cs: ;
    schema:citation "https://www.gida-global.org/care"^^xsd:anyURI ;
.

:f962d3c0-b94d-4306-9c47-f1c430509101
    a skos:Concept ;
    rdfs:isDefinedBy cs: ;
    skos:definition "An item included in a catalogue. Each resource is described with metadata."@en ;
    skos:inScheme cs: ;
    skos:prefLabel "Resource"@en ;
    skos:topConceptOf cs: ;
.

:57110a82-2f4a-4038-aa71-4bbbc888aac4
    a skos:Concept ;
    rdfs:isDefinedBy cs: ;
    skos:definition "Persons or organisations that have a role associated with a resource."@en ;
    skos:inScheme cs: ;
    skos:narrower :c22de8ec-914d-46c9-8c70-3c859765f43e ;
    skos:prefLabel "Agents"@en ;
    skos:topConceptOf cs: ;
.

:6c014466-c95f-4df5-a6cc-a1a50beffab0
    a skos:Concept ;
    rdfs:isDefinedBy cs: ;
    skos:altLabel "PID@en"@en ;
    skos:definition "A unique identifier given to a resource for long term reference."@en ;
    skos:inScheme cs: ;
    skos:narrower :a5cac5df-9d31-4f06-bf2a-fc32bb403e6c ;
    skos:prefLabel "Persistent Identifier"@en ;
    skos:topConceptOf cs: ;
.

<https://linked.data.gov.au/org/idn>
    a
        schema:Organization ,
        schema:Person ;
    schema:email ""^^xsd:anyURI ;
    schema:name "Idn" ;
    schema:url ""^^xsd:anyURI ;
.

cs:
    a skos:ConceptScheme ;
    owl:versionIRI "None" ;
    skos:definition "Glossary of terms describing the Indigenous Data Network metadata profile, guides, specifications and tools."@en ;
    skos:hasTopConcept
        :021c5daa-1354-4dd5-b8cf-8eb112e09174 ,
        :2cab7bd9-8e6d-408b-8120-58ebf0953607 ,
        :324b9d70-1d31-450a-bc5e-a91ab7d65875 ,
        :37258c00-fea6-4837-8b3c-db9efa85a4e3 ,
        :37e0be20-e754-4f7c-a7c8-cb769e3b8d9d ,
        :3e4ebd2a-a787-44c7-b8b9-697e91df313d ,
        :57110a82-2f4a-4038-aa71-4bbbc888aac4 ,
        :5876f61f-1c82-4ac8-894b-b2bfc4debf8d ,
        :61ee574a-e34e-4636-8d6f-5d7ce5807528 ,
        :63da5279-8772-4f9c-8e55-6f5f6f85129a ,
        :6ac34814-bd33-44ce-a1e9-5c71e88f8d06 ,
        :6c014466-c95f-4df5-a6cc-a1a50beffab0 ,
        :6d0f3fed-3187-4825-ad06-35956922dada ,
        :6f057945-b9b9-41ac-b7c1-8eb739bee9fa ,
        :81b2c6f3-1e8c-4a81-ab3b-7949dfc53456 ,
        :87931538-66e5-493d-800f-3c8a54fb8d6b ,
        :8949db57-af31-47fb-a089-b0a77e3feb0e ,
        :9c8ca3b5-cf7d-4c73-83c1-c5c7e5cabb9f ,
        :a06424dd-4d26-4f01-85ee-ca8ff5dfc641 ,
        :a877b16b-2581-4339-9da4-87774b14980a ,
        :ac5eba92-55dc-494c-9d9f-b331e05e7c8d ,
        :c44493ef-8c87-4e41-ac6d-2a0961203a07 ,
        :d7907201-7eaa-4c08-80e1-404c3c2af5c1 ,
        :df76959d-d915-4ce6-9bc8-8043dabc0cc2 ,
        :e1d0f465-d5a9-4154-a241-60c187e825e2 ,
        :f962d3c0-b94d-4306-9c47-f1c430509101 ;
    skos:historyNote "This glossary is developed to assist ongoing operation of the Indigenous Data Network."@en ;
    skos:prefLabel "Indigenous Data Network Glossary"@en ;
    prov:qualifiedAttribution
        [
            dcat:hadRole isoroles:custodian ;
            prov:agent <https://linked.data.gov.au/org/idn> ;
        ] ;
    schema:creator
        [
            a schema:Organization ;
            schema:name "Kurrawong AI" ;
			schema:url "https://kurrawong.ai"^^xsd:anyURI ;
        ] ;
    schema:dateCreated "2024-11-25"^^xsd:date ;
    schema:dateModified "2024-11-26"^^xsd:date ;
    schema:publisher <https://linked.data.gov.au/org/idn> ;
    schema:version "0.1" ;
.
