PREFIX : <https://data.idnau.org/pid/vocab/cat-roles/>
PREFIX cs: <https://data.idnau.org/pid/vocab/cat-roles>
PREFIX dcterms: <http://purl.org/dc/terms/>
PREFIX prov: <http://www.w3.org/ns/prov#>
PREFIX rdfs: <http://www.w3.org/2000/01/rdf-schema#>
PREFIX reg: <http://purl.org/linked-data/registry#>
PREFIX schema: <https://schema.org/>
PREFIX skos: <http://www.w3.org/2004/02/skos/core#>
PREFIX xsd: <http://www.w3.org/2001/XMLSchema#>

:home
    a skos:Concept ;
    dcterms:provenance "Created for the IDN project, 2023"@en ;
    rdfs:isDefinedBy cs: ;
    skos:definition "A catalogue for a resource that is considered to house its point-of-true information" ;
    skos:inScheme cs: ;
    skos:prefLabel "Home"@en ;
    skos:scopeNote "This classification is orthogonal to original/non-original" ;
.

:non-home
    a skos:Concept ;
    dcterms:provenance "Created for the IDN project, 2023"@en ;
    rdfs:isDefinedBy cs: ;
    skos:definition "A catalogue for a resource that is not considered to house its point-of-true information" ;
    skos:inScheme cs: ;
    skos:prefLabel "Non-Home"@en ;
    skos:scopeNote "This classification is orthogonal to original/non-original" ;
.

:non-original
    a skos:Concept ;
    dcterms:provenance "Created for the IDN project, 2023"@en ;
    rdfs:isDefinedBy cs: ;
    skos:definition "An catalogue for a resource that is not the one that first published it" ;
    skos:inScheme cs: ;
    skos:prefLabel "Non-Original"@en ;
    skos:scopeNote "This classification is orthogonal to home/non-home" ;
.

:original
    a skos:Concept ;
    dcterms:provenance "Created for the IDN project, 2023"@en ;
    rdfs:isDefinedBy cs: ;
    skos:definition "An catalogue for a resource that is the one that first published it"@en ;
    skos:inScheme cs: ;
    skos:prefLabel "Original"@en ;
    skos:scopeNote "This classification is orthogonal to home/non-home" ;
.

<https://linked.data.gov.au/org/idn>
    a schema:Organization ;
    schema:name "Indigenous Data Network" ;
    schema:url "https://www.idnau.org"^^xsd:anyURI ;
.

cs:
    a skos:ConceptScheme ;
    dcterms:created "2023-01-17"^^xsd:date ;
    dcterms:creator <https://linked.data.gov.au/org/idn> ;
    dcterms:license "https://creativecommons.org/licenses/by/4.0/"^^xsd:anyURI ;
    dcterms:modified "2023-01-17"^^xsd:date ;
    dcterms:provenance "This vocabulary was established to assist the IDN with differentiating resources' various catalogues. There seems to be no precedent for this form of catalogue classification elsewhere."@en ;
    dcterms:publisher <https://linked.data.gov.au/org/idn> ;
    dcterms:rights "(c) Indigenous Data Network, 2022" ;
    reg:status <https://linked.data.gov.au/def/reg-statuses/experimental> ;
    skos:definition "The Indigenous Data Network's classifications of the roles that Catalogs may play with respect to Resources catalogued within them"@en ;
    skos:hasTopConcept
        :home ,
        :non-home ,
        :non-original ,
        :original ;
    skos:prefLabel "Catalogue Roles"@en ;
    skos:scopeNote """The Concepts in the vocab should be used with qualified dcterms:isPartOf/dcterms:hasPart relations between Resources and Catalogs, e.g.

    {RESOURCE}
        dcterms:isPartOf [
        dcat:hadRole :home ;
        prov:entity {CATALOG} ;
    ] ;
    """ ;
    prov:qualifiedDerivation [
        prov:entity cs: ;
        prov:hadRole <https://linked.data.gov.au/def/vocdermods/none> ;
    ] ;
.
