PREFIX : <https://linked.data.gov.au/def/data-roles/>
PREFIX cs: <https://linked.data.gov.au/def/data-roles>
PREFIX idn: <https://linked.data.gov.au/org/idn>
PREFIX iso: <https://def.isotc211.org/common/RoleCode/>
PREFIX isovoc: <https://def.isotc211.org/common/RoleCode>
PREFIX prov: <http://www.w3.org/ns/prov#>
PREFIX rdfs: <http://www.w3.org/2000/01/rdf-schema#>
PREFIX schema: <https://schema.org/>
PREFIX skos: <http://www.w3.org/2004/02/skos/core#>
PREFIX status: <https://linked.data.gov.au/def/reg-statuses/>
PREFIX xsd: <http://www.w3.org/2001/XMLSchema#>

idn: a schema:Organization ;
    schema:description "The Indigenous Data Network (IDN) was established in 2018 to support and coordinate the governance of Indigenous data for Aboriginal and Torres Strait Islander peoples and empower Aboriginal and Torres Strait Islander communities to decide their own local data priorities."@en ;
    schema:name "Indigenous Data Network" ;
    schema:url "https://mspgh.unimelb.edu.au/centres-institutes/centre-for-health-equity/research-group/indigenous-data-network"^^xsd:anyURI .

:isoRoles a skos:Collection ;
    rdfs:isDefinedBy cs: ;
    skos:definition "Role Codes presented in the ISO 19115 original standard's codelist"@en ;
    skos:historyNote "The list of Concepts from the original ISO 19115 Role Code codelist"@en ;
    skos:inScheme cs: ;
    skos:member iso:author,
        iso:coAuthor,
        iso:collaborator,
        iso:contributor,
        iso:custodian,
        iso:distributor,
        iso:editor,
        iso:funder,
        iso:mediator,
        iso:originator,
        iso:owner,
        iso:pointOfContact,
        iso:principalInvestigator,
        iso:processor,
        iso:publisher,
        iso:resourceProvider,
        iso:rightsHolder,
        iso:sponsor,
        iso:stakeholder,
        iso:user ;
    skos:prefLabel "ISO CI Role Code codes"@en ;
    prov:wasDerivedFrom isovoc: .

:datasteward a skos:Concept ;
    rdfs:isDefinedBy cs: ;
    skos:altLabel "data officer"@en ;
    skos:definition "party responsible for day-to day operations of a catalogue or dataset."@en ;
    skos:historyNote "Created for the Indigenous Data Network's Catalogue Project, 2025"@en ;
    skos:inScheme cs: ;
    skos:prefLabel "data steward"@en ;
    skos:topConceptOf cs: ;
    schema:contributor idn: ;
    schema:status status:addition .

:projectLead a skos:Concept ;
    rdfs:isDefinedBy cs: ;
    skos:definition "party that manages and coordinates responsibility for a research activity."@en ;
    skos:historyNote "Created for the Indigenous Data Network's Catalogue Project, 2025"@en ;
    skos:inScheme cs: ;
    skos:prefLabel "project lead"@en ;
    skos:topConceptOf cs: ;
    schema:contributor idn: ;
    schema:status status:addition .

:projectParticipant a skos:Concept ;
    rdfs:isDefinedBy cs: ;
    skos:definition "party that undertakes a research activity."@en ;
    skos:historyNote "Created for the Indigenous Data Network's Catalogue Project, 2025"@en ;
    skos:inScheme cs: ;
    skos:prefLabel "project participant"@en ;
    skos:topConceptOf cs: ;
    schema:contributor idn: ;
    schema:status status:addition .

:sme a skos:Concept ;
    rdfs:isDefinedBy cs: ;
    skos:altLabel "SME"@en ;
    skos:definition "party responsible for informing practices impacting relevant domain."@en ;
    skos:historyNote "Created for the Indigenous Data Network's Catalogue Project, 2025"@en ;
    skos:inScheme cs: ;
    skos:prefLabel "subject matter expert"@en ;
    skos:topConceptOf cs: ;
    schema:contributor idn: ;
    schema:status status:addition .

:subjectAgent a skos:Concept ;
    rdfs:isDefinedBy cs: ;
    skos:definition "party that the resources contains information about" ;
    skos:historyNote "Created for the Indigenous Data Network's Catalogue Project, 2022"@en ;
    skos:inScheme cs: ;
    skos:prefLabel "subject agent"@en ;
    skos:topConceptOf cs: ;
    schema:contributor idn: ;
    schema:status status:addition .

:subjectAgentRepresentative a skos:Concept ;
    rdfs:isDefinedBy cs: ;
    skos:broader :stakeholder ;
    skos:definition "party who can be contacted who best represents the interests of the subject agent" ;
    skos:historyNote "Created for the Indigenous Data Network's Catalogue Project, 2022"@en ;
    skos:inScheme cs: ;
    skos:prefLabel "subject agent representative"@en ;
    schema:contributor idn: ;
    schema:status status:addition .

:supervisor a skos:Concept ;
    rdfs:isDefinedBy cs: ;
    skos:definition "party that guides and oversees the planning, execution, and completion of a studentâ€™s independent research project, such as an honours thesis, doctoral dissertation, or postdoctoral study."@en ;
    skos:historyNote "Created for the Indigenous Data Network's Catalogue Project, 2025"@en ;
    skos:inScheme cs: ;
    skos:prefLabel "supervisor"@en ;
    skos:topConceptOf cs: ;
    schema:contributor idn: ;
    schema:status status:addition .

:systemadmin a skos:Concept ;
    rdfs:isDefinedBy cs: ;
    skos:altLabel "technical steward"@en ;
    skos:definition "party responsible for an information systems and technologies that support it."@en ;
    skos:historyNote "Created for the Indigenous Data Network's Catalogue Project, 2025"@en ;
    skos:inScheme cs: ;
    skos:prefLabel "system administrator"@en ;
    skos:topConceptOf cs: ;
    schema:contributor idn: ;
    schema:status status:addition .

<https://linked.data.gov.au/org/agldwg> a schema:Organization ;
    schema:description "The Australian Government's community of practice for Linked Data"@en ;
    schema:email "linkeddatairi@ardc.edu.au"^^xsd:anyURI ;
    schema:name "Australian Government Linked Data Working Group" ;
    schema:url "https://www.linked.data.gov.au"^^xsd:anyURI .

iso:author a skos:Concept ;
    rdfs:isDefinedBy isovoc: ;
    skos:definition "party who authored the resource" ;
    skos:historyNote "Presented in the ISO 19115 original standard's codelist"@en ;
    skos:inScheme cs: ;
    skos:prefLabel "author"@en ;
    skos:topConceptOf cs: ;
    schema:status status:original .

iso:coAuthor a skos:Concept ;
    rdfs:isDefinedBy isovoc: ;
    skos:definition "party who jointly authors the resource" ;
    skos:historyNote "Presented in the ISO 19115 original standard's codelist"@en ;
    skos:inScheme cs: ;
    skos:prefLabel "co author"@en ;
    skos:topConceptOf cs: ;
    schema:status status:original .

iso:collaborator a skos:Concept ;
    rdfs:isDefinedBy isovoc: ;
    skos:definition "party who assists with the generation of the resource other than the principal investigator" ;
    skos:historyNote "Presented in the ISO 19115 original standard's codelist"@en ;
    skos:inScheme cs: ;
    skos:prefLabel "collaborator"@en ;
    skos:topConceptOf cs: ;
    schema:status status:original .

iso:contributor a skos:Concept ;
    rdfs:isDefinedBy isovoc: ;
    skos:definition "party contributing to the resource" ;
    skos:historyNote "Presented in the ISO 19115 original standard's codelist"@en ;
    skos:inScheme cs: ;
    skos:prefLabel "contributor"@en ;
    skos:topConceptOf cs: ;
    schema:status status:original .

iso:custodian a skos:Concept ;
    rdfs:isDefinedBy isovoc: ;
    skos:definition "party that accepts accountability and responsibility for the resource and ensures appropriate care and maintenance of the resource" ;
    skos:historyNote "Presented in the ISO 19115 original standard's codelist"@en ;
    skos:inScheme cs: ;
    skos:prefLabel "custodian"@en ;
    skos:topConceptOf cs: ;
    schema:status status:original .

iso:distributor a skos:Concept ;
    rdfs:isDefinedBy isovoc: ;
    skos:definition "party who distributes the resource" ;
    skos:historyNote "Presented in the ISO 19115 original standard's codelist"@en ;
    skos:inScheme cs: ;
    skos:prefLabel "distributor"@en ;
    skos:topConceptOf cs: ;
    schema:status status:original .

iso:editor a skos:Concept ;
    rdfs:isDefinedBy isovoc: ;
    skos:definition "party who reviewed or modified the resource to improve the content" ;
    skos:historyNote "Presented in the ISO 19115 original standard's codelist"@en ;
    skos:inScheme cs: ;
    skos:prefLabel "editor"@en ;
    skos:topConceptOf cs: ;
    schema:status status:original .

iso:funder a skos:Concept ;
    rdfs:isDefinedBy isovoc: ;
    skos:definition "party providing monetary support for the resource" ;
    skos:historyNote "Presented in the ISO 19115 original standard's codelist"@en ;
    skos:inScheme cs: ;
    skos:prefLabel "funder"@en ;
    skos:topConceptOf cs: ;
    schema:status status:original .

iso:mediator a skos:Concept ;
    rdfs:isDefinedBy isovoc: ;
    skos:definition "a class of entity that mediates access to the resource and for whom the resource is intended or useful" ;
    skos:historyNote "Presented in the ISO 19115 original standard's codelist"@en ;
    skos:inScheme cs: ;
    skos:prefLabel "mediator"@en ;
    skos:topConceptOf cs: ;
    schema:status status:original .

iso:originator a skos:Concept ;
    rdfs:isDefinedBy isovoc: ;
    skos:definition "party who created the resource" ;
    skos:historyNote "Presented in the ISO 19115 original standard's codelist"@en ;
    skos:inScheme cs: ;
    skos:prefLabel "originator"@en ;
    skos:topConceptOf cs: ;
    schema:status status:original .

iso:owner a skos:Concept ;
    rdfs:isDefinedBy isovoc: ;
    skos:definition "party that owns the resource" ;
    skos:historyNote "Presented in the ISO 19115 original standard's codelist"@en ;
    skos:inScheme cs: ;
    skos:prefLabel "owner"@en ;
    skos:topConceptOf cs: ;
    schema:status status:original .

iso:pointOfContact a skos:Concept ;
    rdfs:isDefinedBy isovoc: ;
    skos:definition "party who can be contacted for acquiring knowledge about or acquisition of the resource" ;
    skos:historyNote "Presented in the ISO 19115 original standard's codelist"@en ;
    skos:inScheme cs: ;
    skos:prefLabel "point of contact"@en ;
    skos:topConceptOf cs: ;
    schema:status status:original .

iso:principalInvestigator a skos:Concept ;
    rdfs:isDefinedBy isovoc: ;
    skos:definition "key party responsible for gathering information and conducting research" ;
    skos:historyNote "Presented in the ISO 19115 original standard's codelist"@en ;
    skos:inScheme cs: ;
    skos:prefLabel "principal investigator"@en ;
    skos:topConceptOf cs: ;
    schema:status status:original .

iso:processor a skos:Concept ;
    rdfs:isDefinedBy isovoc: ;
    skos:definition "party who has processed the data in a manner such that the resource has been modified" ;
    skos:historyNote "Presented in the ISO 19115 original standard's codelist"@en ;
    skos:inScheme cs: ;
    skos:prefLabel "processor"@en ;
    skos:topConceptOf cs: ;
    schema:status status:original .

iso:publisher a skos:Concept ;
    rdfs:isDefinedBy isovoc: ;
    skos:definition "party who published the resource" ;
    skos:historyNote "Presented in the ISO 19115 original standard's codelist"@en ;
    skos:inScheme cs: ;
    skos:prefLabel "publisher"@en ;
    skos:topConceptOf cs: ;
    schema:status status:original .

iso:resourceProvider a skos:Concept ;
    rdfs:isDefinedBy isovoc: ;
    skos:definition "party that supplies the resource" ;
    skos:historyNote "Presented in the ISO 19115 original standard's codelist"@en ;
    skos:inScheme cs: ;
    skos:prefLabel "resource provider"@en ;
    skos:topConceptOf cs: ;
    schema:status status:original .

iso:rightsHolder a skos:Concept ;
    rdfs:isDefinedBy isovoc: ;
    skos:definition "party owning or managing rights over the resource" ;
    skos:historyNote "Presented in the ISO 19115 original standard's codelist"@en ;
    skos:inScheme cs: ;
    skos:prefLabel "rights holder"@en ;
    skos:topConceptOf cs: ;
    schema:status status:original .

iso:sponsor a skos:Concept ;
    rdfs:isDefinedBy isovoc: ;
    skos:definition "party who speaks for the resource" ;
    skos:historyNote "Presented in the ISO 19115 original standard's codelist"@en ;
    skos:inScheme cs: ;
    skos:prefLabel "sponsor"@en ;
    skos:topConceptOf cs: ;
    schema:status status:original .

iso:stakeholder a skos:Concept ;
    rdfs:isDefinedBy isovoc: ;
    skos:definition "party who has an interest in the resource or the use of the resource" ;
    skos:historyNote "Presented in the ISO 19115 original standard's codelist"@en ;
    skos:inScheme cs: ;
    skos:prefLabel "stakeholder"@en ;
    skos:topConceptOf cs: ;
    schema:status status:original .

iso:user a skos:Concept ;
    rdfs:isDefinedBy isovoc: ;
    skos:definition "party who uses the resource" ;
    skos:historyNote "Presented in the ISO 19115 original standard's codelist"@en ;
    skos:inScheme cs: ;
    skos:prefLabel "user"@en ;
    skos:topConceptOf cs: ;
    schema:status status:original .

cs: a skos:ConceptScheme ;
    skos:definition "This vocabulary lists the roles that Agents - People and Organisations - play in relation to data. This is an extended and Semantic Web version of the International Organisation for Standardization's ISO19115-1 standard's Role Codes codelist."@en ;
    skos:hasTopConcept iso:author,
        iso:coAuthor,
        iso:collaborator,
        iso:contributor,
        iso:custodian,
        iso:distributor,
        iso:editor,
        iso:funder,
        iso:mediator,
        iso:originator,
        iso:owner,
        iso:pointOfContact,
        iso:principalInvestigator,
        iso:processor,
        iso:publisher,
        iso:resourceProvider,
        iso:rightsHolder,
        iso:sponsor,
        iso:stakeholder,
        iso:user,
        :datasteward,
        :projectLead,
        :projectParticipant,
        :sme,
        :subjectAgent,
        :subjectAgentRepresentative,
        :supervisor,
        :systemadmin ;
    skos:historyNote "Derived from the ISO 19115's CI Role Code codelist and added to by Australian vocabulary users"@en ;
    skos:prefLabel "IDN Role Codes"@en ;
    prov:qualifiedDerivation [ a prov:Derivation ;
            prov:entity cs: ;
            prov:hadRole <https://linked.data.gov.au/def/vocdermods/none> ] ;
    schema:citation "http://iso.kurrawong.net/vocab/CI_RoleCode"^^xsd:anyURI ;
    schema:copyrightNotice "(c) Australian Government Linked Data Working Group, 2024" ;
    schema:creator idn: ;
    schema:dateCreated "2024-02-28"^^xsd:date ;
    schema:dateIssued "2024-02-28"^^xsd:date ;
    schema:dateModified "2025-08-26"^^xsd:date ;
    schema:license "https://creativecommons.org/licenses/by/4.0/"^^xsd:anyURI ;
    schema:publisher <https://linked.data.gov.au/org/agldwg> ;
    schema:status status:stable .

