PREFIX : <https://data.idnau.org/pid/vocab/idn-glossary/>
PREFIX cs: <https://data.idnau.org/pid/vocab/idn-glossary>
PREFIX owl: <http://www.w3.org/2002/07/owl#>
PREFIX rdfs: <http://www.w3.org/2000/01/rdf-schema#>
PREFIX schema: <https://schema.org/>
PREFIX skos: <http://www.w3.org/2004/02/skos/core#>
PREFIX xsd: <http://www.w3.org/2001/XMLSchema#>

<https://linked.data.gov.au/org/idn>
    a schema:Organization ;
    schema:name "Indigenous Data Network" ;
    schema:url "https://www.idnau.org"^^xsd:anyURI ;
.

:aps
    a skos:Concept ;
    skos:historyNote "Created in 2025 by IDN from different sources"@en ;
    rdfs:isDefinedBy cs: ;
    skos:altLabel "APS"@en ;
    skos:definition "The Australian Public Service (APS) comprises entities that employ their staff under the Public Service Act 1999 (PS Act). This includes all departments of state, and some other entities. Generally, APS agencies are ‘non-corporate’, being components of the legal entity that is the Commonwealth."@en ;
    skos:inScheme cs: ;
    skos:prefLabel "Australian Public Sector"@en ;
    skos:topConceptOf cs: ;
.

:ird
    a skos:Concept ;
    skos:historyNote "Created in 2025 by IDN from different sources"@en ;
    rdfs:isDefinedBy cs: ;
    skos:definition "Within this project, we refer to Indigenous research data as all data generated by, about or for Aboriginal and Torres Strait Islander people in Australia. Indigenous research data specifically refers to information that is collected, analysed, and interpreted within the context of Indigenous communities, cultures, and knowledge systems. It includes data gathered through research projects conducted by and with Indigenous peoples, as well as data that Indigenous communities have generated and maintained themselves. Indigenous research data includes traditional ecological knowledge, oral histories, cultural practices, and other forms of Indigenous knowledge that may not fit traditional Western research paradigms. It may involve collaborative research approaches that prioritise Indigenous self-determination, community engagement, and the equitable sharing of benefits."@en ;
    skos:inScheme cs: ;
    skos:prefLabel "Indigenous research data"@en ;
    skos:topConceptOf cs: ;
.

:idc
    a skos:Concept ;
    skos:historyNote "Created in 2025 by IDN from different sources"@en ;
    rdfs:isDefinedBy cs: ;
    skos:altLabel "IDC"@en ;
    skos:definition """For the purposes of the IIRC Project, we define Indigenous Data Custodians as five broad communities of Indigenous research data custodians:
(1) Aboriginal and Torres Strait Islander communities and organisations;
(2) universities, researchers and other research organisations;
(3) the GLAM sector, including libraries, archives and museums;
(4) Commonwealth, state, territory and local governments; and
(5) Private sector (including not-for-profit)."""@en ;
    skos:inScheme cs: ;
    skos:prefLabel "Indigenous Data Custodian"@en ;
    skos:topConceptOf cs: ;
.

:idg
    a skos:Concept ;
    skos:historyNote "Created in 2025 by IDN from different sources"@en ;
    rdfs:isDefinedBy cs: ;
    skos:altLabel "IDG"@en ;
    skos:definition """Indigenous data governance refers to the principles, practices, and systems by which Indigenous communities exercise control over the collection, ownership, management, and use of data that is relevant to them. It recognises the unique rights, interests, and needs of Indigenous peoples regarding their data and aims to ensure that data is collected, stored, and utilised in a manner that respects their self-determination, cultural values, and sovereignty.

Indigenous data governance sets the foundations for data democracy at the community level, supporting Indigenous access, generation, and use of data."""@en ;
    skos:inScheme cs: ;
    skos:prefLabel "Indigenous Data Governance"@en ;
    skos:topConceptOf cs: ;
.

:ids
    a skos:Concept ;
    skos:historyNote "Created in 2025 by IDN from different sources"@en ;
    rdfs:isDefinedBy cs: ;
    skos:altLabel "IDS"@en ;
    skos:definition "Indigenous data sovereignty refers to the right of Indigenous communities to own, control, and govern the data that is generated within their communities. It encompasses the principles of self-determination, cultural autonomy, and control over information and knowledge systems."@en ;
    skos:inScheme cs: ;
    skos:prefLabel "Indigenous Data Sovereignty"@en ;
    skos:topConceptOf cs: ;
.

:idnc
    a skos:Concept ;
    skos:historyNote "Created in 2025 by IDN from different sources"@en ;
    rdfs:isDefinedBy cs: ;
    skos:altLabel "IDNC"@en ;
    skos:definition "The Indigenous Data Network's catalogue of Indigenous datasets includes metadata of Indigenous data held by IDCs across Australia, including research data generated by the IDN in partnership with IDCs. This catalogue will be built over time as metadata of significant Indigenous datasets are located. The IDNC demonstrates improved metadata models and rating systems for data and metadata to improve Indigenous Data Governance."@en ;
    skos:inScheme cs: ;
    skos:prefLabel "Indigenous Data Network Catalogue"@en ;
    skos:topConceptOf cs: ;
.

cs:
    a skos:ConceptScheme ;
    schema:dateCreated "2025-10-15"^^xsd:date ;
    schema:creator <https://linked.data.gov.au/org/idn> ;
    schema:dateIssued "2026-01-30"^^xsd:date ;
    schema:license "https://creativecommons.org/licenses/by/4.0/"^^xsd:anyURI ;
    schema:dateModified "2026-01-30"^^xsd:date ;
    skos:historyNote "Created in 2025 by IDN from different sources"@en ;
    schema:publisher <https://linked.data.gov.au/org/idn> ;
    schema:copyrightNotice "(c) Indigenous Data Network, 2026" ;
    owl:versionIRI :0.0.1 ;
    owl:versionInfo "0.0.1" ;
    skos:definition "IDN terms defined for use via the IDN's website at https://idnau.org/resources/glossary"@en ;
    skos:hasTopConcept
        :aps  ,
        :ird  ,
        :idc  ,
        :idg  ,
        :ids  ,
        :idnc ;
    skos:prefLabel "IDN Glossary"@en ;
.

:0.0.1 schema:name "0.0.1" .