PREFIX : <https://data.idnau.org/pid/glossary/>
PREFIX cs: <https://data.idnau.org/pid/glossary>
PREFIX drole: <https://linked.data.gov.au/def/data-roles/>
PREFIX dcat: <http://www.w3.org/ns/dcat#>
PREFIX dcterms: <http://purl.org/dc/terms/>
PREFIX idn: <https://linked.data.gov.au/org/idn>
PREFIX kai: <https://kurrawong.ai>
PREFIX prov: <http://www.w3.org/ns/prov#>
PREFIX rdfs: <http://www.w3.org/2000/01/rdf-schema#>
PREFIX regstat: <https://linked.data.gov.au/def/reg-statuses/>
PREFIX schema: <https://schema.org/>
PREFIX skos: <http://www.w3.org/2004/02/skos/core#>
PREFIX xsd: <http://www.w3.org/2001/XMLSchema#>

:bd5028a2-8536-4ca3-bef8-1525790271f7
    a skos:Concept ;
    dcterms:source "https://idnau.org/resources/glossary"^^xsd:anyURI ;
    skos:inScheme cs: ;
    skos:topConceptOf cs: ;
    skos:prefLabel "Indigenous research data"@en ;
    skos:definition "Within the IDN project, we refer to Indigenous research data as all data generated by, about or for Aboriginal and Torres Strait Islander people in Australia. Indigenous research data specifically refers to information that is collected, analysed, and interpreted within the context of Indigenous communities, cultures, and knowledge systems. It includes data gathered through research projects conducted by and with Indigenous peoples, as well as data that Indigenous communities have generated and maintained themselves. Indigenous research data includes traditional ecological knowledge, oral histories, cultural practices, and other forms of Indigenous knowledge that may not fit traditional Western research paradigms. It may involve collaborative research approaches that prioritise Indigenous self-determination, community engagement, and the equitable sharing of benefits."@en
.

:b6360ba0-c76d-4d47-85f6-1df8a475d7f7
    a skos:Concept ;
    dcterms:source "https://idnau.org/resources/glossary"^^xsd:anyURI ;
    skos:inScheme cs: ;
    skos:topConceptOf cs: ;
    skos:prefLabel "Indigenous Data Custodian"@en ;
    skos:altLabel "IDC"@en ;
    skos:definition """For the purposes of the IIRC Project, we define Indigenous Data Custodians as five broad communities of Indigenous research data custodians:
(1) Aboriginal and Torres Strait Islander communities and organisations;
(2) universities, researchers and other research organisations;
(3) the GLAM sector, including libraries, archives and museums;
(4) Commonwealth, state, territory and local governments; and
(5) Private sector (including not-for-profit)."""@en
.

:4532385d-a41a-4a19-b2a7-1b5af48c4cf0
    a skos:Concept ;
    dcterms:source "https://idnau.org/resources/glossary"^^xsd:anyURI ;
    skos:inScheme cs: ;
    skos:topConceptOf cs: ;
    skos:prefLabel "Indigenous Data Governance"@en ;
    skos:altLabel "IDG"@en ;
    skos:definition "Within the IDN project, we refer to Indigenous research data as all data generated by, about or for Aboriginal and Torres Strait Islander people in Australia. Indigenous research data specifically refers to information that is collected, analysed, and interpreted within the context of Indigenous communities, cultures, and knowledge systems. It includes data gathered through research projects conducted by and with Indigenous peoples, as well as data that Indigenous communities have generated and maintained themselves. Indigenous research data includes traditional ecological knowledge, oral histories, cultural practices, and other forms of Indigenous knowledge that may not fit traditional Western research paradigms. It may involve collaborative research approaches that prioritise Indigenous self-determination, community engagement, and the equitable sharing of benefits."@en
.

:4434bc6d-a7c3-4787-9069-7ee01a057b31
    a skos:Concept ;
    dcterms:source "https://idnau.org/resources/glossary"^^xsd:anyURI ;
    skos:inScheme cs: ;
    skos:topConceptOf cs: ;
    skos:prefLabel "Indigenous Data Sovereignty"@en ;
    skos:altLabel "IDS"@en ;
    skos:definition "Indigenous data sovereignty refers to the right of Indigenous communities to own, control, and govern the data that is generated within their communities. It encompasses the principles of self-determination, cultural autonomy, and control over information and knowledge systems."@en
.

:021c5daa-1354-4dd5-b8cf-8eb112e09174
    a skos:Concept ;
    rdfs:isDefinedBy cs: ;
    skos:definition "Tracking changes to resources over time."@en ;
    skos:inScheme cs: ;
    skos:prefLabel "Versioning"@en ;
    skos:topConceptOf cs: ;
.

:2cab7bd9-8e6d-408b-8120-58ebf0953607
    a skos:Concept ;
    rdfs:isDefinedBy cs: ;
    skos:definition "A resource is accessible if it is possible to get a resource by a persistant identifier, or to get information about how to get the resource."@en ;
    skos:inScheme cs: ;
    skos:prefLabel "Accessible"@en ;
    skos:topConceptOf cs: ;
.

:324b9d70-1d31-450a-bc5e-a91ab7d65875
    a skos:Concept ;
    rdfs:isDefinedBy cs: ;
    skos:altLabel "RDF"@en ;
    skos:definition "A type of metadata for describing resources on the internet."@en ;
    skos:inScheme cs: ;
    skos:prefLabel "Resource Description Framework"@en ;
    skos:topConceptOf cs: ;
    schema:citation "https://www.w3.org/TR/rdf11-concepts/"^^xsd:anyURI ;
.

:37258c00-fea6-4837-8b3c-db9efa85a4e3
    a skos:Concept ;
    rdfs:isDefinedBy cs: ;
    skos:definition "A tool that checks if metadata conforms to the rules of a profile."@en ;
    skos:inScheme cs: ;
    skos:prefLabel "Validator"@en ;
    skos:topConceptOf cs: ;
    schema:citation "https://www.w3.org/TR/shacl/#dfn-validators/"^^xsd:anyURI ;
.

:37e0be20-e754-4f7c-a7c8-cb769e3b8d9d
    a skos:Concept ;
    rdfs:isDefinedBy cs: ;
    skos:definition "A set of rules or guidelines for creating consistent metadata."@en ;
    skos:inScheme cs: ;
    skos:prefLabel "Profile"@en ;
    skos:topConceptOf cs: ;
.

:3e4ebd2a-a787-44c7-b8b9-697e91df313d
    a skos:Concept ;
    rdfs:isDefinedBy cs: ;
    skos:altLabel
        "Catalog"@en ,
        "Data catalogue"@en ;
    skos:definition "A collection of metadata records organised for easy access and use."@en ;
    skos:inScheme cs: ;
    skos:prefLabel "Catalogue"@en ;
    skos:topConceptOf cs: ;
.

:5876f61f-1c82-4ac8-894b-b2bfc4debf8d
    a skos:Concept ;
    rdfs:isDefinedBy cs: ;
    skos:altLabel "Interoperable"@en ;
    skos:definition "The ability to share information between different collections or catalogues that might use different tools."@en ;
    skos:inScheme cs: ;
    skos:prefLabel "Interoperability"@en ;
    skos:topConceptOf cs: ;
.

:61ee574a-e34e-4636-8d6f-5d7ce5807528
    a skos:Concept ;
    rdfs:isDefinedBy cs: ;
    skos:altLabel "JavaScript Object Notation for Linked Data"@en ;
    skos:definition "A method for storing and sharing Resource Description Framework metadata."@en ;
    skos:inScheme cs: ;
    skos:prefLabel "JSON-LD"@en ;
    skos:topConceptOf cs: ;
    schema:citation "https://json-ld.org"^^xsd:anyURI ;
.

:63da5279-8772-4f9c-8e55-6f5f6f85129a
    a skos:Concept ;
    rdfs:isDefinedBy cs: ;
    skos:definition "Metadata about the relationships between things."@en ;
    skos:inScheme cs: ;
    skos:prefLabel "Ontology"@en ;
    skos:topConceptOf cs: ;
    schema:citation "https://doi.org/10.1006/knac.1993.1008"^^xsd:anyURI ;
.

:6ac34814-bd33-44ce-a1e9-5c71e88f8d06
    a skos:Concept ;
    rdfs:isDefinedBy cs: ;
    skos:definition "Principles to make resources Findable, Accessible, Interoperable, and Reusable."@en ;
    skos:inScheme cs: ;
    skos:prefLabel "FAIR principles"@en ;
    skos:topConceptOf cs: ;
    schema:citation "https://www.go-fair.org/fair-principles/"^^xsd:anyURI ;
.

:6d0f3fed-3187-4825-ad06-35956922dada
    a skos:Concept ;
    rdfs:isDefinedBy cs: ;
    skos:altLabel
        "Concept scheme"@en ,
        "Controlled vocabulary"@en ;
    skos:definition "A set of predefined words or phrases used for describing metadata records consistently."@en ;
    skos:inScheme cs: ;
    skos:prefLabel "Vocabulary"@en ;
    skos:topConceptOf cs: ;
.

:6f057945-b9b9-41ac-b7c1-8eb739bee9fa
    a skos:Concept ;
    rdfs:isDefinedBy cs: ;
    skos:altLabel "DCAT"@en ;
    skos:definition "A standard used for describing data catalogs on the web to enable interoperability between systems."@en ;
    skos:inScheme cs: ;
    skos:prefLabel "Data Catalog Vocabulary"@en ;
    skos:topConceptOf cs: ;
    schema:citation "https://www.w3.org/TR/vocab-dcat-3/"^^xsd:anyURI ;
.

:81b2c6f3-1e8c-4a81-ab3b-7949dfc53456
    a skos:Concept ;
    rdfs:isDefinedBy cs: ;
    skos:definition "A resource is reuseable if there is permission from those responsible for the resource to use it."@en ;
    skos:inScheme cs: ;
    skos:prefLabel "Reuseable"@en ;
    skos:topConceptOf cs: ;
.

:87931538-66e5-493d-800f-3c8a54fb8d6b
    a skos:Concept ;
    rdfs:isDefinedBy cs: ;
    skos:definition "The prefix of an identifier that groups concepts or resources together."@en ;
    skos:inScheme cs: ;
    skos:prefLabel "Namespace"@en ;
    skos:topConceptOf cs: ;
.

:8949db57-af31-47fb-a089-b0a77e3feb0e
    a skos:Concept ;
    rdfs:isDefinedBy cs: ;
    skos:definition "Information that describes a resource, such as its title, description, author or custodian."@en ;
    skos:inScheme cs: ;
    skos:prefLabel "Metadata"@en ;
    skos:topConceptOf cs: ;
.

:9c8ca3b5-cf7d-4c73-83c1-c5c7e5cabb9f
    a skos:Concept ;
    rdfs:isDefinedBy cs: ;
    skos:altLabel
        "TTL"@en ,
        "Terse RDF Triple Language"@en ;
    skos:definition "A method for storing and sharing Resource Description Framework metadata."@en ;
    skos:inScheme cs: ;
    skos:prefLabel "Turtle"@en ;
    skos:topConceptOf cs: ;
    schema:citation "https://www.w3.org/TR/turtle/"^^xsd:anyURI ;
.

:a06424dd-4d26-4f01-85ee-ca8ff5dfc641
    a skos:Concept ;
    rdfs:isDefinedBy cs: ;
    skos:definition "The relationship between people or organisations and catalogued resources."@en ;
    skos:inScheme cs: ;
    skos:prefLabel "Role"@en ;
    skos:topConceptOf cs: ;
.

:a5cac5df-9d31-4f06-bf2a-fc32bb403e6c
    a skos:Concept ;
    rdfs:isDefinedBy cs: ;
    skos:altLabel "UUID"@en ;
    skos:broader :6c014466-c95f-4df5-a6cc-a1a50beffab0 ;
    skos:definition "A type of persistant identifier that is universally unique."@en ;
    skos:inScheme cs: ;
    skos:prefLabel "Universally Unique Identifier"@en ;
.

:a877b16b-2581-4339-9da4-87774b14980a
    a skos:Concept ;
    rdfs:isDefinedBy cs: ;
    skos:altLabel
        "BC labels"@en ,
        "Bicultural labels"@en ,
        "LC labels"@en ,
        "Traditional knowledge labels"@en ;
    skos:definition "Conepts that express local and specific conditions such as community rules, governance and protocols for using and sharing knowledge."@en ;
    skos:inScheme cs: ;
    skos:prefLabel "Local context labels"@en ;
    skos:topConceptOf cs: ;
    schema:citation "https://localcontexts.org/labels/traditional-knowledge-labels/"^^xsd:anyURI ;
.

:ac5eba92-55dc-494c-9d9f-b331e05e7c8d
    a skos:Concept ;
    rdfs:isDefinedBy cs: ;
    skos:definition "A single unit of meaning or part of knowledge. Conepts are expressed as words or terms. Many concepts from the same knowledge system belong to a vocabulary."@en ;
    skos:inScheme cs: ;
    skos:prefLabel "Concept"@en ;
    skos:topConceptOf cs: ;
    schema:citation "https://www.w3.org/TR/skos-reference/#concepts"^^xsd:anyURI ;
.

:c44493ef-8c87-4e41-ac6d-2a0961203a07
    a skos:Concept ;
    rdfs:isDefinedBy cs: ;
    skos:altLabel "Metadata tool"@en ;
    skos:definition "A tool that helps to create and upload metadata about resources."@en ;
    skos:inScheme cs: ;
    skos:prefLabel "Metadata Entry Form" ;
    skos:topConceptOf cs: ;
    schema:url "https://metadata.idnau.org/"^^xsd:anyURI ;
.

:d7907201-7eaa-4c08-80e1-404c3c2af5c1
    a skos:Concept ;
    rdfs:isDefinedBy cs: ;
    skos:definition "A resource is findable if it is possible to find that resource. Resources are findable when they are described with consistent metadata and vocabulary concepts."@en ;
    skos:inScheme cs: ;
    skos:prefLabel "Findable"@en ;
    skos:topConceptOf cs: ;
.

:df76959d-d915-4ce6-9bc8-8043dabc0cc2
    a skos:Concept ;
    rdfs:isDefinedBy cs: ;
    skos:altLabel "Qualified attribution"@en ;
    skos:definition "Metadata about the agent and the role that they played with respect to a resource."@en ;
    skos:inScheme cs: ;
    skos:prefLabel "Attribution"@en ;
    skos:topConceptOf cs: ;
.

:e1d0f465-d5a9-4154-a241-60c187e825e2
    a skos:Concept ;
    rdfs:isDefinedBy cs: ;
    skos:definition "Priniples for the ethical use and sharing of data to prioritize community benefit, agency, and respect. They are: Collective Benefit; Authority to Control; Responsibility; Ethics."@en ;
    skos:inScheme cs: ;
    skos:prefLabel "CARE Principles"@en ;
    skos:topConceptOf cs: ;
    schema:citation "https://www.gida-global.org/care"^^xsd:anyURI ;
.

:f962d3c0-b94d-4306-9c47-f1c430509101
    a skos:Concept ;
    rdfs:isDefinedBy cs: ;
    skos:definition "An item included in a catalogue. Each resource is described with metadata."@en ;
    skos:inScheme cs: ;
    skos:prefLabel "Resource"@en ;
    skos:topConceptOf cs: ;
.

<https://kurrawong.ai>
    a schema:Organization ;
    schema:name "KurrawongAI" ;
    schema:url "https://kurrawong.ai"^^xsd:anyURI ;
.

:57110a82-2f4a-4038-aa71-4bbbc888aac4
    a skos:Concept ;
    rdfs:isDefinedBy cs: ;
    skos:definition "Persons or organisations that have a role associated with a resource."@en ;
    skos:inScheme cs: ;
    skos:narrowMatch drole:subjectAgent ;
    skos:prefLabel "Agents"@en ;
    skos:topConceptOf cs: ;
.

:6c014466-c95f-4df5-a6cc-a1a50beffab0
    a skos:Concept ;
    rdfs:isDefinedBy cs: ;
    skos:altLabel "PID"@en ;
    skos:definition "A unique identifier given to a resource for long term reference."@en ;
    skos:inScheme cs: ;
    skos:narrower :a5cac5df-9d31-4f06-bf2a-fc32bb403e6c ;
    skos:prefLabel "Persistent Identifier"@en ;
    skos:topConceptOf cs: ;
.

:66c85faf-5624-45b9-ae7a-49f8fe7f1f84
    a skos:Concept ;
    prov:wasDerivedFrom drole:subjectAgent ;
    skos:broadMatch :57110a82-2f4a-4038-aa71-4bbbc888aac4 ;
    skos:definition "Person or organisation that the resource is about."@en ;
    skos:historyNote "This concept is taken from the Data roles vocabulary."@en ;
    skos:inScheme cs: ;
    skos:prefLabel "Subject agent"@en ;
.

idn:
    a schema:Organization ;
    schema:name "Indigenous Data Network" ;
    schema:url "https://www.idnau.org"^^xsd:anyURI ;
.

cs:
    a skos:ConceptScheme ;
    schema:status regstat:experimental ;
    skos:definition "Glossary of terms describing the Indigenous Data Network metadata profile, guides, specifications and tools."@en ;
    skos:hasTopConcept
        :021c5daa-1354-4dd5-b8cf-8eb112e09174 ,
        :2cab7bd9-8e6d-408b-8120-58ebf0953607 ,
        :324b9d70-1d31-450a-bc5e-a91ab7d65875 ,
        :37258c00-fea6-4837-8b3c-db9efa85a4e3 ,
        :37e0be20-e754-4f7c-a7c8-cb769e3b8d9d ,
        :3e4ebd2a-a787-44c7-b8b9-697e91df313d ,
        :57110a82-2f4a-4038-aa71-4bbbc888aac4 ,
        :5876f61f-1c82-4ac8-894b-b2bfc4debf8d ,
        :61ee574a-e34e-4636-8d6f-5d7ce5807528 ,
        :63da5279-8772-4f9c-8e55-6f5f6f85129a ,
        :6ac34814-bd33-44ce-a1e9-5c71e88f8d06 ,
        :6c014466-c95f-4df5-a6cc-a1a50beffab0 ,
        :6d0f3fed-3187-4825-ad06-35956922dada ,
        :6f057945-b9b9-41ac-b7c1-8eb739bee9fa ,
        :81b2c6f3-1e8c-4a81-ab3b-7949dfc53456 ,
        :87931538-66e5-493d-800f-3c8a54fb8d6b ,
        :8949db57-af31-47fb-a089-b0a77e3feb0e ,
        :9c8ca3b5-cf7d-4c73-83c1-c5c7e5cabb9f ,
        :a06424dd-4d26-4f01-85ee-ca8ff5dfc641 ,
        :a877b16b-2581-4339-9da4-87774b14980a ,
        :ac5eba92-55dc-494c-9d9f-b331e05e7c8d ,
        :c44493ef-8c87-4e41-ac6d-2a0961203a07 ,
        :d7907201-7eaa-4c08-80e1-404c3c2af5c1 ,
        :df76959d-d915-4ce6-9bc8-8043dabc0cc2 ,
        :e1d0f465-d5a9-4154-a241-60c187e825e2 ,
        :f962d3c0-b94d-4306-9c47-f1c430509101 ;
    skos:historyNote "This glossary is developed to assist ongoing operation of the Indigenous Data Network."@en ;
    skos:prefLabel "Indigenous Data Network Glossary"@en ;
    prov:qualifiedAttribution
        [
            dcat:hadRole drole:custodian ;
            prov:agent idn: ;
        ] ;
    schema:creator kai: ;
    schema:dateCreated "2024-11-25"^^xsd:date ;
    schema:dateModified "2025-12-29"^^xsd:date ;
    schema:publisher idn: ;
    schema:version "0.2" ;
.
