PREFIX : <https://data.idnau.org/pid/vocab/indigeneity/>
PREFIX cs: <https://data.idnau.org/pid/vocab/indigeneity>
PREFIX dcterms: <http://purl.org/dc/terms/>
PREFIX prov: <http://www.w3.org/ns/prov#>
PREFIX rdfs: <http://www.w3.org/2000/01/rdf-schema#>
PREFIX reg: <http://purl.org/linked-data/registry#>
PREFIX schema: <https://schema.org/>
PREFIX skos: <http://www.w3.org/2004/02/skos/core#>
PREFIX xsd: <http://www.w3.org/2001/XMLSchema#>

:about-indigenous-people
    a skos:Concept ;
    dcterms:provenance "Created for the IDN project, 2022"@en ;
    rdfs:isDefinedBy cs: ;
    skos:definition "Data that is about indigenous people" ;
    skos:inScheme cs: ;
    skos:prefLabel "About Indigenous People"@en ;
.

:about-indigenous-things
    a skos:Concept ;
    dcterms:provenance "Created for the IDN project, 2022"@en ;
    rdfs:isDefinedBy cs: ;
    skos:definition "Data that is about indigenous things; land, resources, knowledge etc." ;
    skos:inScheme cs: ;
    skos:prefLabel "About Indigenous Things"@en ;
.

:by-indigenous-people
    a skos:Concept ;
    dcterms:provenance "Created for the IDN project, 2022"@en ;
    rdfs:isDefinedBy cs: ;
    skos:definition "Data that is created/published or in some other way by indigenous people" ;
    skos:inScheme cs: ;
    skos:prefLabel "By Indigenous People"@en ;
.

<https://linked.data.gov.au/org/idn>
    a schema:Organization ;
    schema:description "The Indigenous Data Network (IDN) was established in 2018 to support and coordinate the governance of Indigenous data for Aboriginal and Torres Strait Islander peoples and empower Aboriginal and Torres Strait Islander communities to decide their own local data priorities."@en ;
    schema:name "Indigenous Data Network" ;
    schema:url "https://mspgh.unimelb.edu.au/centres-institutes/centre-for-health-equity/research-group/indigenous-data-network"^^xsd:anyURI ;
.

cs:
    a skos:ConceptScheme ;
    dcterms:created "2022-08-29"^^xsd:date ;
    dcterms:creator <https://linked.data.gov.au/org/idn> ;
    dcterms:license "https://creativecommons.org/licenses/by/4.0/"^^xsd:anyURI ;
    dcterms:modified "2022-08-29"^^xsd:date ;
    dcterms:publisher <https://linked.data.gov.au/org/idn> ;
    dcterms:rights "(c) Indigenous Data Network, 2022" ;
    dcterms:source "https://www.data.govt.nz/assets/Uploads/Presentation-Tahu-Kukutai.pdf"^^xsd:anyURI ;
    reg:status <https://linked.data.gov.au/def/reg-statuses/experimental> ;
    skos:definition "The ways in which data may have a connection to indigenous people"@en ;
    skos:hasTopConcept
        :about-indigenous-people ,
        :about-indigenous-things ,
        :by-indigenous-people ;
    skos:prefLabel "Data Indigeneity"@en ;
    skos:scopeNote "The IDN uses this vocabulary to indicate how, if at all, data is related to indigenous people. This is a simple vocabulary that is expected to be extended in later versions."@en ;
    prov:qualifiedDerivation [
        prov:entity cs: ;
        prov:hadRole <https://linked.data.gov.au/def/vocdermods/none> ;
    ] ;
.
